More on compare function
 - Optimized implementation in GenTree for AVL and RBT
 - Some facts in Facts.OrdProperties, and a final OrderedMaps module
 - Remove Interface.Sord
 - Btw, eq_key and eq_key_elt replaced by generic Fst and Duo.

Comparisons.v
@@ -12,6 +12,56 @@ Set Implicit Arguments.
 Notation "c1 >>= c2" :=
   (match c1 with Lt => Lt | Gt => Gt | Eq => c2 end) (at level 70).
 
+(** The comparison function in OrderedType are symmetric and
+    transitive in the following sense: *)
+
+Definition Sym {A} (cmp:A->A->comparison) :=
+  forall x y, cmp y x = CompOpp (cmp x y).
+
+Definition Trans {A} (cmp:A->A->comparison) :=
+  forall c x y z, cmp x y = c -> cmp y z = c -> cmp x z = c.
+
+Class SymTrans {A} (cmp:A->A->comparison) := {
+  sym :> Sym cmp;
+  tra :> Trans cmp
+}.
+
+(** [SymTrans] implies the following compatibility rules *)
+
+Definition CompatR {A} (cmp:A->A->comparison) :=
+  forall x y y', cmp y y' = Eq -> cmp x y = cmp x y'.
+
+Definition CompatL {A} (cmp:A->A->comparison) :=
+  forall x x' y, cmp x x' = Eq -> cmp x y = cmp x' y.
+
+Ltac flipcmp H :=
+ match type of H with ?cmp _ _ = _ =>
+   match goal with
+   | Sy : Sym cmp |- _ => rewrite Sy, CompOpp_iff in H; simpl in H
+   | Sy : SymTrans cmp |- _ => rewrite sym, CompOpp_iff in H; simpl in H
+   end
+ end.
+
+Lemma SymTrans_CompatR {A} (cmp:A->A->comparison) :
+  SymTrans cmp -> CompatR cmp.
+Proof.
+ intros (Sy,Tr) x y y' Hy.
+ destruct (cmp x y) eqn:E, (cmp x y') eqn:E'; trivial.
+ - erewrite Tr in E'; eauto.
+ - erewrite Tr in E'; eauto.
+ - erewrite Tr in E; eauto. now flipcmp Hy.
+ - flipcmp E. erewrite Tr in Hy; eauto. easy.
+ - flipcmp Hy. erewrite Tr in E; eauto.
+ - flipcmp E. erewrite Tr in Hy; eauto. easy.
+Qed.
+
+Lemma SymTrans_CompatL {A} (cmp:A->A->comparison) :
+  SymTrans cmp -> CompatL cmp.
+Proof.
+ intros ST x x' y Hx. rewrite (sym y x), (sym y x'). f_equal.
+ apply SymTrans_CompatR; auto.
+Qed.
+
 (** Lexicographic comparison on pairs *)
 
 Section PairComp.
@@ -19,6 +69,44 @@ Variable A B : Type.
 Variable cmpA : A -> A -> comparison.
 Variable cmpB : B -> B -> comparison.
 Definition pair_compare '(a,b) '(a',b') := cmpA a a' >>= cmpB b b'.
+
+Lemma pair_compare_sym : Sym cmpA -> Sym cmpB -> Sym pair_compare.
+Proof.
+ intros HA HB (x,x') (y,y'). simpl.
+ rewrite HA, HB. destruct cmpA; simpl; auto.
+Qed.
+
+Lemma pair_compare_trans :
+  SymTrans cmpA -> Trans cmpB -> Trans pair_compare.
+Proof.
+ intros HA HB c (x,x') (y,y') (z,z') Hxy Hyz. simpl in *.
+ destruct (cmpA x y) eqn:Cxy; simpl.
+ - rewrite SymTrans_CompatL; eauto.
+   destruct (cmpA y z) eqn:Cyz; simpl; eauto.
+ - subst c.
+   destruct (cmpA y z) eqn:Cyz; simpl; try easy.
+   + flipcmp Cyz. rewrite SymTrans_CompatR, Cxy; eauto.
+   + rewrite tra; eauto. easy.
+ - subst c.
+   destruct (cmpA y z) eqn:Cyz; simpl; try easy.
+   + flipcmp Cyz. rewrite SymTrans_CompatR, Cxy; eauto.
+   + rewrite tra; eauto. easy.
+Qed.
+
+Global Instance pair_compare_st :
+  SymTrans cmpA -> SymTrans cmpB -> SymTrans pair_compare.
+Proof.
+ constructor.
+ - apply pair_compare_sym; apply sym.
+ - apply pair_compare_trans; auto. apply tra.
+Qed.
+
+Lemma pair_compare_eq a a' b b' :
+  pair_compare (a,b) (a',b') = Eq <-> cmpA a a' = Eq /\ cmpB b b' = Eq.
+Proof.
+ simpl. destruct cmpA; split; try easy.
+Qed.
+
 End PairComp.
 
 (** Comparison on lists *)
@@ -33,4 +121,42 @@ Fixpoint list_compare (l1 l2 : list A) :=
   | _, [] => Gt
   | x1::l1', x2::l2' => cmp x1 x2 >>= list_compare l1' l2'
   end.
+
+Lemma list_compare_sym : Sym cmp -> Sym list_compare.
+Proof.
+ intros HA. red. induction x as [|a x IH]; destruct y as [|a' y]; auto.
+ simpl. rewrite HA. destruct cmp; simpl; auto.
+Qed.
+
+Lemma list_compare_trans :
+  SymTrans cmp -> Trans list_compare.
+Proof.
+ intros HA c.
+ induction x as [|a x IH]; destruct y as [|a' y], z as [|a'' z];
+  simpl; auto; try congruence.
+ destruct (cmp a a') eqn:E, (cmp a' a'') eqn:E'; simpl; try congruence.
+ - rewrite tra; eauto. simpl; eauto.
+ - intros _ <-. rewrite SymTrans_CompatL, E'; eauto.
+ - intros _ <-. rewrite SymTrans_CompatL, E'; eauto.
+ - intros <- _. rewrite SymTrans_CompatR, E; eauto. now flipcmp E'.
+ - intros <- _. rewrite tra; eauto. easy.
+ - intros <- _. rewrite SymTrans_CompatR, E; eauto. now flipcmp E'.
+ - intros <- _. rewrite tra; eauto. easy.
+Qed.
+
+Global Instance list_compare_st : SymTrans cmp -> SymTrans list_compare.
+Proof.
+ constructor. apply list_compare_sym, sym. now apply list_compare_trans.
+Qed.
+
+Lemma list_compare_eq l l' :
+  list_compare l l' = Eq <-> Forall2 (fun a a' => cmp a a' = Eq) l l'.
+Proof.
+ split.
+ - revert l'.
+   induction l as [|a l IH]; destruct l' as [|b l']; simpl; try easy.
+   destruct (cmp a b) eqn:E; auto; try easy.
+ - induction 1; simpl; auto. now rewrite H.
+Qed.
+
 End ListComp.
